Rework all_pcs to account for alignment

compiler/encoders/asm/asmPropsScript.sml
@@ -65,21 +65,24 @@ val target_ok_def = Define`
 val interference_ok_def = Define `
   interference_ok env proj <=> !i:num ms. proj (env i ms) = proj ms`;
 
-val all_pcs_def = Define `
-  (all_pcs 0 a = {}) /\
-  (all_pcs (SUC n) a = a INSERT all_pcs n (a + 1w))`
+val all_pcs_def = Define`
+  (all_pcs 0 a k = {}) ∧
+  (all_pcs n a k = a INSERT all_pcs (n-(MAX 1 k)) (a + n2w (MAX 1 k)) k)`;
 
 val all_pcs_thm = Q.store_thm("all_pcs_thm",
-  `all_pcs x y = IMAGE (((+) y) o n2w) (count x)`,
-  qid_spec_tac`y`
-  \\ Induct_on`x`
-  \\ rw[all_pcs_def]
+  `all_pcs n a k = { a + n2w (i * (MAX 1 k)) | i | i * (MAX 1 k) < n }`,
+  qid_spec_tac`a`
+  \\ qid_spec_tac`k`
+  \\ completeInduct_on`n`
+  \\ Cases_on`n` \\ rw[all_pcs_def]
   \\ rw[EXTENSION]
-  \\ qmatch_goalsub_rename_tac`a = y`
-  \\ Cases_on`a = y` \\ fs[]
+  \\ Cases_on`a = x` \\ fs[]
   >- ( qexists_tac`0` \\ fs[] )
   \\ rewrite_tac[word_add_n2w,GSYM WORD_ADD_ASSOC,GSYM ADD1]
-  \\ METIS_TAC[LESS_MONO_EQ,prim_recTheory.INV_SUC_EQ,WORD_ADD_0,num_CASES]);
+  \\ rw[EQ_IMP_THM]
+  >- ( qexists_tac`SUC i` \\ simp[ADD1,LEFT_ADD_DISTRIB,RIGHT_ADD_DISTRIB] )
+  \\ qexists_tac`i-1`
+  \\ Cases_on`i` \\ fs[ADD1,LEFT_ADD_DISTRIB,RIGHT_ADD_DISTRIB]);
 
 val asserts_def = zDefine `
   (asserts 0 next ms _ Q <=> Q (next 0 ms)) /\
@@ -96,8 +99,8 @@ val backend_correct_def = Define `
             let pcs = all_pcs (LENGTH (t.config.encode i)) s1.pc in
             asserts n (\k s. env (n - k) (t.next s)) ms
               (\ms'. t.state_ok ms' /\
-                     (∀pc. pc ∈ pcs ⇒ t.get_byte ms' pc = t.get_byte ms pc) ∧
-                     t.get_pc ms' IN pcs)
+                     (∀pc. pc ∈ pcs 1 ⇒ t.get_byte ms' pc = t.get_byte ms pc) ∧
+                     t.get_pc ms' IN pcs t.config.code_alignment)
               (\ms'. target_state_rel t s2 ms')`
 
 (* lemma for proofs *)
@@ -115,8 +118,31 @@ val bytes_in_memory_APPEND = Q.store_thm("bytes_in_memory_APPEND",
   )
 
 val bytes_in_memory_all_pcs = Q.store_thm("bytes_in_memory_all_pcs",
-  `!xs pc. bytes_in_memory pc xs m d ==> all_pcs (LENGTH xs) pc SUBSET d`,
-  Induct \\ full_simp_tac(srw_ss())[all_pcs_def,bytes_in_memory_def]);
+  `!xs pc. bytes_in_memory pc xs m d ==> all_pcs (LENGTH xs) pc k SUBSET d`,
+  gen_tac
+  \\ completeInduct_on`LENGTH xs`
+  \\ rw[]
+  \\ fs[all_pcs_thm]
+  \\ fs[SUBSET_DEF, PULL_EXISTS, PULL_FORALL] \\ rw[]
+  \\ Cases_on`i=0` \\ fs[]
+  >- ( Cases_on`xs` \\ fs[bytes_in_memory_def] )
+  \\ Cases_on`MAX 1 k < LENGTH xs`
+  >- (
+    first_x_assum(qspec_then`DROP (MAX 1 k) xs`mp_tac)
+    \\ simp[]
+    \\ Q.ISPECL_THEN[`TAKE (MAX 1 k) xs`,`DROP (MAX 1 k) xs`]mp_tac bytes_in_memory_APPEND
+    \\ simp[]
+    \\ disch_then(drule o #1 o EQ_IMP_RULE o SPEC_ALL)
+    \\ strip_tac
+    \\ disch_then drule
+    \\ disch_then(qspec_then`i-1`mp_tac)
+    \\ simp[LEFT_SUB_DISTRIB, RIGHT_SUB_DISTRIB]
+    \\ rewrite_tac[GSYM WORD_ADD_ASSOC]
+    \\ rewrite_tac[word_add_n2w]
+    \\ simp[SUB_LEFT_ADD]
+    \\ IF_CASES_TAC \\ fs[]
+    \\ `i = 1` by fs[] \\ fs[] )
+  \\ Cases_on`i` \\ fs[ADD1, RIGHT_ADD_DISTRIB, MAX_DEF]);
 
 val bytes_in_memory_change_domain = Q.store_thm("bytes_in_memory_change_domain",
   `∀a bs m md1 md2.
